src/tests/pars.fs
@@ -35,9 +35,8 @@ let init_once () : unit =
   let env = TcEnv.initial_env Tc.type_of Tc.universe_of solver Const.prims_lid in
   env.solver.init env;
   let dsenv, prims_mod = parse_prims () in
-//  let env = 
-//  let prims_mod, env = Tc.check_module env prims_mod in
-//  let env = TcEnv.set_current_module env test_lid in
+  let prims_mod, env = Tc.check_module env prims_mod in
+  let env = TcEnv.set_current_module env test_lid in
   tcenv_ref := Some env
 
 let rec init () = 
