ulib/prims.fst
@@ -178,445 +178,443 @@ effect Admit (a:Type) = PURE a (fun (p:pure_post a) -> True)
 (* The primitive effect Tot is definitionally equal to an instance of PURE *)
 effect Tot (a:Type) = PURE a (pure_null_wp a)
 
-(* total new_effect GHOST = PURE *)
-#set-options "--debug_level Norm --debug_level Extreme --print_bound_var_types --print_implicits"
+total new_effect GHOST = PURE
 inline let purewp_id (a:Type) (wp:pure_wp a) = wp
 
-(* sub_effect *)
-(*   PURE ~> GHOST = purewp_id *)
-
-(* (\* The primitive effect GTot is definitionally equal to an instance of GHOST *\) *)
-(* effect GTot (a:Type) = GHOST a (pure_null_wp a) *)
-(* (\* #set-options "--print_universes --print_implicits --print_bound_var_types --debug Prims --debug_level Extreme" *\) *)
-(* effect Ghost (a:Type) (pre:Type) (post:pure_post a) = *)
-(*        GHOST a *)
-(*            (fun (p:pure_post a) -> pre /\ (forall (x:a). post x ==> p x)) *)
-
-(* assume new type int : Type0 *)
-
-(* assume HasEq_int: hasEq int *)
-
-(* assume val op_AmpAmp             : bool -> bool -> Tot bool *)
-(* assume val op_BarBar             : bool -> bool -> Tot bool *)
-(* assume val op_Negation           : bool -> Tot bool *)
-(* assume val op_Multiply           : int -> int -> Tot int *)
-(* assume val op_Subtraction        : int -> int -> Tot int *)
-(* assume val op_Addition           : int -> int -> Tot int *)
-(* assume val op_Minus              : int -> Tot int *)
-(* assume val op_LessThanOrEqual    : int -> int -> Tot bool *)
-(* assume val op_GreaterThan        : int -> int -> Tot bool *)
-(* assume val op_GreaterThanOrEqual : int -> int -> Tot bool *)
-(* assume val op_LessThan           : int -> int -> Tot bool *)
-(* assume val op_Equality :    #a:Type{hasEq a} -> a -> a -> Tot bool *)
-(* assume val op_disEquality : #a:Type{hasEq a} -> a -> a -> Tot bool *)
-(* assume new type exn : Type0 *)
-(* assume new type array : Type -> Type0 *)
-(* assume val strcat : string -> string -> Tot string *)
-
-(* assume HasEq_string: hasEq string *)
-
-(* type list (a:Type) = *)
-(*   | Nil  : list a *)
-(*   | Cons : hd:a -> tl:list a -> list a *)
-
-(* assume HasEq_list: (forall (a:Type).{:pattern (hasEq (list a))} hasEq a ==> hasEq (list a)) *)
-
-(* type pattern = *)
-(*   | SMTPat   : #a:Type -> a -> pattern *)
-(*   | SMTPatT  : a:Type0 -> pattern  *)
-(*   | SMTPatOr : list (list pattern) -> pattern  *)
-
-(* assume type decreases : #a:Type -> a -> Type0 *)
-
-(* (\* *)
-(*    Lemma is desugared specially. You can write: *)
-
-(*      Lemma phi                 for   Lemma (requires True) phi [] *)
-(*      Lemma t1..tn              for   Lemma unit t1..tn *)
-(* *\) *)
-(* effect Lemma (a:Type) (pre:Type) (post:Type) (pats:list pattern) = *)
-(*        Pure a pre (fun r -> post) *)
-
-
-(* type option (a:Type) = *)
-(*   | None : option a *)
-(*   | Some : v:a -> option a *)
-
-(* assume HasEq_option: (forall (a:Type).{:pattern (hasEq (option a))} hasEq a ==> hasEq (option a)) *)
-
-(* type either 'a 'b = *)
-(*   | Inl : v:'a -> either 'a 'b *)
-(*   | Inr : v:'b -> either 'a 'b *)
-
-(* assume HasEq_either: (forall (a:Type) (b:Type).{:pattern (hasEq (either a b))} (hasEq a /\ hasEq b) ==> hasEq (either a b)) *)
-
-(* type result (a:Type) = *)
-(*   | V   : v:a -> result a *)
-(*   | E   : e:exn -> result a *)
-(*   | Err : msg:string -> result a *)
-
-(* (\* This new bit for Dijkstra Monads for Free; it has a "double meaning", *)
-(*  * either as an alias for reasoning about the direct definitions, or as a marker *)
-(*  * for places where a CPS transformation should happen. *\) *)
-(* effect M (a:Type) = Tot a *)
-
-(* assume HasEq_result: (forall (a:Type).{:pattern (hasEq (result a))} hasEq a ==> hasEq (result a)) *)
-
-(* new_effect DIV = PURE *)
-(* sub_effect PURE ~> DIV  = purewp_id *)
-
-(* effect Div (a:Type) (pre:pure_pre) (post:pure_post a) = *)
-(*        DIV a *)
-(*            (fun (p:pure_post a) -> pre /\ (forall a. pre /\ post a ==> p a)) (\* WP *\) *)
-
-(* effect Dv (a:Type) = *)
-(*      DIV a (fun (p:pure_post a) -> (forall (x:a). p x)) *)
-
-
-(* let st_pre_h  (heap:Type)          = heap -> GTot Type0 *)
-(* let st_post_h (heap:Type) (a:Type) = a -> heap -> GTot Type0 *)
-(* let st_wp_h   (heap:Type) (a:Type) = st_post_h heap a -> Tot (st_pre_h heap) *)
-
-(* inline let st_return        (heap:Type) (a:Type) *)
-(*                             (x:a) (p:st_post_h heap a) = *)
-(*      p x *)
-(* inline let st_bind_wp       (heap:Type)  *)
-(* 			    (r1:range)  *)
-(* 			    (a:Type) (b:Type) *)
-(*                             (wp1:st_wp_h heap a) *)
-(*                             (wp2:(a -> GTot (st_wp_h heap b))) *)
-(*                             (p:st_post_h heap b) (h0:heap) = *)
-(*      labeled r1 "push" unit *)
-(*      /\ wp1 (fun a h1 -> *)
-(*        labeled r1 "pop" unit *)
-(*        /\ wp2 a p h1) h0 *)
-(* inline let st_if_then_else  (heap:Type) (a:Type) (p:Type) *)
-(*                              (wp_then:st_wp_h heap a) (wp_else:st_wp_h heap a) *)
-(*                              (post:st_post_h heap a) (h0:heap) = *)
-(*      l_ITE p *)
-(*         (wp_then post h0) *)
-(* 	(wp_else post h0) *)
-(* inline let st_ite_wp        (heap:Type) (a:Type) *)
-(*                             (wp:st_wp_h heap a) *)
-(*                             (post:st_post_h heap a) (h0:heap) = *)
-(*      forall (k:st_post_h heap a). *)
-(* 	 (forall (x:a) (h:heap).{:pattern (guard_free (k x h))} k x h <==> post x h) *)
-(* 	 ==> wp k h0 *)
-(* inline let st_stronger  (heap:Type) (a:Type) (wp1:st_wp_h heap a) *)
-(*                         (wp2:st_wp_h heap a) = *)
-(*      (forall (p:st_post_h heap a) (h:heap). wp1 p h ==> wp2 p h) *)
-
-(* inline let st_close_wp      (heap:Type) (a:Type) (b:Type) *)
-(*                              (wp:(b -> GTot (st_wp_h heap a))) *)
-(*                              (p:st_post_h heap a) (h:heap) = *)
-(*      (forall (b:b). wp b p h) *)
-(* inline let st_assert_p      (heap:Type) (a:Type) (p:Type) *)
-(*                              (wp:st_wp_h heap a) *)
-(*                              (q:st_post_h heap a) (h:heap) = *)
-(*      p /\ wp q h *)
-(* inline let st_assume_p      (heap:Type) (a:Type) (p:Type) *)
-(*                              (wp:st_wp_h heap a) *)
-(*                              (q:st_post_h heap a) (h:heap) = *)
-(*      p ==> wp q h *)
-(* inline let st_null_wp       (heap:Type) (a:Type) *)
-(*                              (p:st_post_h heap a) (h:heap) = *)
-(*      (forall (x:a) (h:heap). p x h) *)
-(* inline let st_trivial       (heap:Type) (a:Type) *)
-(*                              (wp:st_wp_h heap a) = *)
-(*      (forall h0. wp (fun r h1 -> True) h0) *)
-
-(* new_effect { *)
-(*   STATE_h (heap:Type) : result:Type -> wp:st_wp_h heap result -> Effect *)
-(*   with return_wp      = st_return heap *)
-(*      ; bind_wp      = st_bind_wp heap *)
-(*      ; if_then_else = st_if_then_else heap *)
-(*      ; ite_wp       = st_ite_wp heap *)
-(*      ; stronger     = st_stronger heap *)
-(*      ; close_wp     = st_close_wp heap *)
-(*      ; assert_p     = st_assert_p heap *)
-(*      ; assume_p     = st_assume_p heap *)
-(*      ; null_wp      = st_null_wp heap *)
-(*      ; trivial      = st_trivial heap *)
-(* } *)
-
-(* (\* Effect EXCEPTION *\) *)
-(* let ex_pre  = Type0 *)
-(* let ex_post (a:Type) = result a -> GTot Type0 *)
-(* let ex_wp   (a:Type) = ex_post a -> GTot ex_pre *)
-(* inline let ex_return   (a:Type) (x:a) (p:ex_post a) : GTot Type0 = p (V x) *)
-(* inline let ex_bind_wp (r1:range) (a:Type) (b:Type) *)
-(* 		       (wp1:ex_wp a) *)
-(* 		       (wp2:(a -> GTot (ex_wp b))) (p:ex_post b) *)
-(*          : GTot Type0 = *)
-(*   forall (k:ex_post b). *)
-(*      (forall (rb:result b).{:pattern (guard_free (k rb))} k rb <==> p rb) *)
-(*      ==> (labeled r1 "push" unit *)
-(*          /\ wp1 (fun ra1 -> labeled r1 "pop" unit *)
-(* 			/\ (is_V ra1 ==> wp2 (V.v ra1) k) *)
-(* 			/\ (is_E ra1 ==> k (E (E.e ra1))))) *)
-
-(* inline let ex_ite_wp (a:Type) (wp:ex_wp a) (post:ex_post a) = *)
-(*   forall (k:ex_post a). *)
-(*      (forall (rb:result a).{:pattern (guard_free (k rb))} k rb <==> post rb) *)
-(*      ==> wp k *)
-
-(* inline let ex_if_then_else (a:Type) (p:Type) (wp_then:ex_wp a) (wp_else:ex_wp a) (post:ex_post a) = *)
-(*    l_ITE p *)
-(*        (wp_then post) *)
-(*        (wp_else post) *)
-(* inline let ex_stronger (a:Type) (wp1:ex_wp a) (wp2:ex_wp a) = *)
-(*         (forall (p:ex_post a). wp1 p ==> wp2 p) *)
-
-(* inline let ex_close_wp (a:Type) (b:Type) (wp:(b -> GTot (ex_wp a))) (p:ex_post a) = (forall (b:b). wp b p) *)
-(* inline let ex_assert_p (a:Type) (q:Type) (wp:ex_wp a) (p:ex_post a) = (q /\ wp p) *)
-(* inline let ex_assume_p (a:Type) (q:Type) (wp:ex_wp a) (p:ex_post a) = (q ==> wp p) *)
-(* inline let ex_null_wp (a:Type) (p:ex_post a) = (forall (r:result a). p r) *)
-(* inline let ex_trivial (a:Type) (wp:ex_wp a) = wp (fun r -> True) *)
-
-(* new_effect { *)
-(*   EXN : result:Type -> wp:ex_wp result -> Effect *)
-(*   with *)
-(*     return_wp    = ex_return *)
-(*   ; bind_wp      = ex_bind_wp *)
-(*   ; if_then_else = ex_if_then_else *)
-(*   ; ite_wp       = ex_ite_wp *)
-(*   ; stronger     = ex_stronger *)
-(*   ; close_wp     = ex_close_wp *)
-(*   ; assert_p     = ex_assert_p *)
-(*   ; assume_p     = ex_assume_p *)
-(*   ; null_wp      = ex_null_wp *)
-(*   ; trivial      = ex_trivial *)
-(* } *)
-(* effect Exn (a:Type) (pre:ex_pre) (post:ex_post a) = *)
-(*        EXN a *)
-(*          (fun (p:ex_post a) -> pre /\ (forall (r:result a). (pre /\ post r) ==> p r)) (\* WP *\) *)
-
-(* inline let lift_div_exn (a:Type) (wp:pure_wp a) (p:ex_post a) = wp (fun a -> p (V a)) *)
-(* sub_effect DIV ~> EXN = lift_div_exn *)
-(* effect Ex (a:Type) = Exn a True (fun v -> True) *)
-
-(* let all_pre_h  (h:Type)           = h -> GTot Type0 *)
-(* let all_post_h (h:Type) (a:Type)  = result a -> h -> GTot Type0 *)
-(* let all_wp_h   (h:Type) (a:Type)  = all_post_h h a -> Tot (all_pre_h h) *)
-
-(* inline let all_ite_wp (heap:Type) (a:Type) *)
-(*                       (wp:all_wp_h heap a) *)
-(*                       (post:all_post_h heap a) (h0:heap) = *)
-(*     forall (k:all_post_h heap a). *)
-(*        (forall (x:result a) (h:heap).{:pattern (guard_free (k x h))} k x h <==> post x h) *)
-(*        ==> wp k h0 *)
-(* inline let all_return  (heap:Type) (a:Type) (x:a) (p:all_post_h heap a) = p (V x) *)
-(* inline let all_bind_wp (heap:Type) (r1:range) (a:Type) (b:Type) *)
-(*                        (wp1:all_wp_h heap a) *)
-(*                        (wp2:(a -> GTot (all_wp_h heap b))) *)
-(*                        (p:all_post_h heap b) (h0:heap) : GTot Type0 = *)
-(*    labeled r1 "push" unit *)
-(*    /\ wp1 (fun ra h1 ->  *)
-(*        labeled r1 "pop" unit *)
-(*        /\ (is_V ra ==> wp2 (V.v ra) p h1)) h0 *)
-
-(* inline let all_if_then_else (heap:Type) (a:Type) (p:Type) *)
-(*                              (wp_then:all_wp_h heap a) (wp_else:all_wp_h heap a) *)
-(*                              (post:all_post_h heap a) (h0:heap) = *)
-(*    l_ITE p *)
-(*        (wp_then post h0) *)
-(*        (wp_else post h0) *)
-(* inline let all_stronger (heap:Type) (a:Type) (wp1:all_wp_h heap a) *)
-(*                         (wp2:all_wp_h heap a) = *)
-(*     (forall (p:all_post_h heap a) (h:heap). wp1 p h ==> wp2 p h) *)
-
-(* inline let all_close_wp (heap:Type) (a:Type) (b:Type) *)
-(*                          (wp:(b -> GTot (all_wp_h heap a))) *)
-(*                          (p:all_post_h heap a) (h:heap) = *)
-(*     (forall (b:b). wp b p h) *)
-(* inline let all_assert_p (heap:Type) (a:Type) (p:Type) *)
-(*                          (wp:all_wp_h heap a) (q:all_post_h heap a) (h:heap) = *)
-(*     p /\ wp q h *)
-(* inline let all_assume_p (heap:Type) (a:Type) (p:Type) *)
-(*                          (wp:all_wp_h heap a) (q:all_post_h heap a) (h:heap) = *)
-(*     p ==> wp q h *)
-(* inline let all_null_wp (heap:Type) (a:Type) *)
-(*                         (p:all_post_h heap a) (h0:heap) = *)
-(*     (forall (a:result a) (h:heap). p a h) *)
-(* inline let all_trivial (heap:Type) (a:Type) (wp:all_wp_h heap a) = *)
-(*     (forall (h0:heap). wp (fun r h1 -> True) h0) *)
-
-(* new_effect { *)
-(*   ALL_h (heap:Type) : a:Type -> wp:all_wp_h heap a -> Effect *)
-(*   with *)
-(*     return_wp    = all_return       heap *)
-(*   ; bind_wp      = all_bind_wp      heap *)
-(*   ; if_then_else = all_if_then_else heap *)
-(*   ; ite_wp       = all_ite_wp       heap *)
-(*   ; stronger     = all_stronger     heap *)
-(*   ; close_wp     = all_close_wp     heap *)
-(*   ; assert_p     = all_assert_p     heap *)
-(*   ; assume_p     = all_assume_p     heap *)
-(*   ; null_wp      = all_null_wp      heap *)
-(*   ; trivial      = all_trivial      heap *)
-(* } *)
-
-
-
-
-
-(* type lex_t = *)
-(*   | LexTop  : lex_t *)
-(*   | LexCons : #a:Type -> a -> lex_t -> lex_t *)
-
-(* (\* 'a * 'b *\) *)
-(* type tuple2 'a 'b = *)
-(*   | Mktuple2: _1:'a *)
-(*            -> _2:'b *)
-(*            -> tuple2 'a 'b *)
-
-(* assume HasEq_tuple2: (forall (a:Type) (b:Type).{:pattern (hasEq (tuple2 a b))} (hasEq a /\ hasEq b) ==> hasEq (tuple2 a b)) *)
-
-(* (\* 'a * 'b * 'c *\) *)
-(* type tuple3 'a 'b 'c = *)
-(*   | Mktuple3: _1:'a *)
-(*            -> _2:'b *)
-(*            -> _3:'c *)
-(*           -> tuple3 'a 'b 'c *)
-
-(* assume HasEq_tuple3: (forall (a:Type) (b:Type) (c:Type).{:pattern (hasEq (tuple3 a b c))} (hasEq a /\ hasEq b /\ hasEq c) ==> hasEq (tuple3 a b c)) *)
-
-(* (\* 'a * 'b * 'c * 'd *\) *)
-(* type tuple4 'a 'b 'c 'd = *)
-(*   | Mktuple4: _1:'a *)
-(*            -> _2:'b *)
-(*            -> _3:'c *)
-(*            -> _4:'d *)
-(*            -> tuple4 'a 'b 'c 'd *)
-
-(* assume HasEq_tuple4: (forall (a:Type) (b:Type) (c:Type) (d:Type).{:pattern (hasEq (tuple4 a b c d))} (hasEq a /\ hasEq b /\ hasEq c /\ hasEq d) ==> hasEq (tuple4 a b c d)) *)
-
-(* (\* 'a * 'b * 'c * 'd * 'e *\) *)
-(* type tuple5 'a 'b 'c 'd 'e = *)
-(*   | Mktuple5: _1:'a *)
-(*            -> _2:'b *)
-(*            -> _3:'c *)
-(*            -> _4:'d *)
-(*            -> _5:'e *)
-(*            -> tuple5 'a 'b 'c 'd 'e *)
-
-(* assume HasEq_tuple5: (forall (a:Type) (b:Type) (c:Type) (d:Type) (e:Type).{:pattern (hasEq (tuple5 a b c d e))} (hasEq a /\ hasEq b /\ hasEq c /\ hasEq d /\ hasEq e) ==> hasEq (tuple5 a b c d e)) *)
-
-(* (\* 'a * 'b * 'c * 'd * 'e * 'f *\) *)
-(* type tuple6 'a 'b 'c 'd 'e 'f = *)
-(*   | Mktuple6: _1:'a *)
-(*            -> _2:'b *)
-(*            -> _3:'c *)
-(*            -> _4:'d *)
-(*            -> _5:'e *)
-(*            -> _6:'f *)
-(*            -> tuple6 'a 'b 'c 'd 'e 'f *)
-
-(* assume HasEq_tuple6: (forall (a:Type) (b:Type) (c:Type) (d:Type) (e:Type) (f:Type).{:pattern (hasEq (tuple6 a b c d e f))} (hasEq a /\ hasEq b /\ hasEq c /\ hasEq d /\ hasEq e /\ hasEq f) ==> hasEq (tuple6 a b c d e f)) *)
-
-(* (\* 'a * 'b * 'c * 'd * 'e * 'f * 'g *\) *)
-(* type tuple7 'a 'b 'c 'd 'e 'f 'g = *)
-(*   | Mktuple7: _1:'a *)
-(*            -> _2:'b *)
-(*            -> _3:'c *)
-(*            -> _4:'d *)
-(*            -> _5:'e *)
-(*            -> _6:'f *)
-(*            -> _7:'g *)
-(*            -> tuple7 'a 'b 'c 'd 'e 'f 'g *)
-
-(* assume HasEq_tuple7: (forall (a:Type) (b:Type) (c:Type) (d:Type) (e:Type) (f:Type) (g:Type).{:pattern (hasEq (tuple7 a b c d e f g))} (hasEq a /\ hasEq b /\ hasEq c /\ hasEq d /\ hasEq e /\ hasEq f /\ hasEq g) ==> hasEq (tuple7 a b c d e f g)) *)
-
-(* (\* 'a * 'b * 'c * 'd * 'e * 'f * 'g * 'h *\) *)
-(* type tuple8 'a 'b 'c 'd 'e 'f 'g 'h = *)
-(*   | Mktuple8: _1:'a *)
-(*            -> _2:'b *)
-(*            -> _3:'c *)
-(*            -> _4:'d *)
-(*            -> _5:'e *)
-(*            -> _6:'f *)
-(*            -> _7:'g *)
-(*            -> _8:'h *)
-(*            -> tuple8 'a 'b 'c 'd 'e 'f 'g 'h *)
-
-(* assume HasEq_tuple8: (forall (a:Type) (b:Type) (c:Type) (d:Type) (e:Type) (f:Type) (g:Type) (h:Type).{:pattern (hasEq (tuple8 a b c d e f g h))} (hasEq a /\ hasEq b /\ hasEq c /\ hasEq d /\ hasEq e /\ hasEq f /\ hasEq g /\ hasEq h) ==> hasEq (tuple8 a b c d e f g h)) *)
-
-(* (\* Concrete syntax (x:a & y:b x & c x y) *\) *)
-(* type dtuple3 (a:Type) *)
-(*              (b:(a -> GTot Type)) *)
-(*              (c:(x:a -> b x -> GTot Type)) = *)
-(*    | Mkdtuple3:_1:a *)
-(*              -> _2:b _1 *)
-(*              -> _3:c _1 _2 *)
-(*              -> dtuple3 a b c *)
-
-(* (\* Concrete syntax (x:a & y:b x & z:c x y & d x y z) *\) *)
-(* type dtuple4 (a:Type) *)
-(*              (b:(x:a -> GTot Type)) *)
-(*              (c:(x:a -> b x -> GTot Type)) *)
-(*              (d:(x:a -> y:b x -> z:c x y -> GTot Type)) = *)
-(*  | Mkdtuple4:_1:a *)
-(*            -> _2:b _1 *)
-(*            -> _3:c _1 _2 *)
-(*            -> _4:d _1 _2 _3 *)
-(*            -> dtuple4 a b c d *)
-
-(* let as_requires (#a:Type) (wp:pure_wp a)  = wp (fun x -> True) *)
-(* let as_ensures  (#a:Type) (wp:pure_wp a) (x:a) = ~ (wp (fun y -> (y=!=x))) *)
-
-(* val fst : ('a * 'b) -> Tot 'a *)
-(* let fst x = Mktuple2._1 x *)
-
-(* val snd : ('a * 'b) -> Tot 'b *)
-(* let snd x = Mktuple2._2 x *)
-
-(* val dfst : #a:Type -> #b:(a -> GTot Type) -> dtuple2 a b -> Tot a *)
-(* let dfst #a #b t = Mkdtuple2._1 t *)
-
-(* val dsnd : #a:Type -> #b:(a -> GTot Type) -> t:dtuple2 a b -> Tot (b (Mkdtuple2._1 t)) *)
-(* let dsnd #a #b t = Mkdtuple2._2 t *)
-
-(* assume val _assume : p:Type -> unit -> Pure unit (requires (True)) (ensures (fun x -> p)) *)
-(* assume val admit   : #a:Type -> unit -> Admit a *)
-(* assume val magic   : #a:Type -> unit -> Tot a *)
-(* irreducible val unsafe_coerce  : #a:Type -> #b: Type -> a -> Tot b *)
-(* let unsafe_coerce #a #b x = admit(); x *)
-(* assume val admitP  : p:Type -> Pure unit True (fun x -> p) *)
-(* assume val _assert : p:Type -> unit -> Pure unit (requires p) (ensures (fun x -> True)) *)
-(* assume val cut     : p:Type -> Pure unit (requires p) (fun x -> p) *)
-(* assume val qintro  : #a:Type -> #p:(a -> GTot Type) -> $f:(x:a -> Lemma (p x)) -> Lemma (forall (x:a). p x) *)
-(* assume val ghost_lemma: #a:Type -> #p:(a -> GTot Type) -> #q:(a -> unit -> GTot Type) -> *)
-(*   $f:(x:a -> Ghost unit (p x) (q x)) -> Lemma (forall (x:a). p x ==> q x ()) *)
-(* assume val raise: exn -> Ex 'a       (\* TODO: refine with the Exn monad *\) *)
-
-
-(* val ignore: #a:Type -> a -> Tot unit *)
-(* let ignore #a x = () *)
-
-(* type nat = i:int{i >= 0} *)
-(* type pos = i:int{i > 0} *)
-(* type nonzero = i:int{i<>0} *)
-
-(* let allow_inversion (a:Type)  *)
-(*   : Pure unit (requires True) (ensures (fun x -> inversion a)) *)
-(*   = () *)
-
-(* (\*    For the moment we require not just that the divisor is non-zero, *\) *)
-(* (\*    but also that the dividend is natural. This works around a *\) *)
-(* (\*    mismatch between the semantics of integer division in SMT-LIB and *\) *)
-(* (\*    in F#/OCaml. For SMT-LIB ints the modulus is always positive (as in *\) *)
-(* (\*    math Euclidian division), while for F#/OCaml ints the modulus has *\) *)
-(* (\*    the same sign as the dividend. Our arbitrary precision ints don't *\) *)
-(* (\*    quite correspond to finite precision F#/OCaml ints though, but to *\) *)
-(* (\*    OCaml's big_ints (for which the modulus is always positive).  So *\) *)
-(* (\*    we'll need to return to this point anyway, when we discuss how to *\) *)
-(* (\*    soundly map F* ints to something in F#/OCaml.  *\) *)
-
-(* assume val op_Modulus            : int -> nonzero -> Tot int *)
-(* assume val op_Division           : nat -> nonzero -> Tot int *)
-
-(* let rec pow2 (x:nat) : Tot pos = if x = 0 then 1 else op_Multiply 2 (pow2 (x-1)) *)
-(* let abs (x:int) : Tot int = if x >= 0 then x else -x *)
-
-(* assume val string_of_bool: bool -> Tot string *)
-(* assume val string_of_int: int -> Tot string *)
+sub_effect
+  PURE ~> GHOST = purewp_id
+
+(* The primitive effect GTot is definitionally equal to an instance of GHOST *)
+effect GTot (a:Type) = GHOST a (pure_null_wp a)
+effect Ghost (a:Type) (pre:Type) (post:pure_post a) =
+       GHOST a
+           (fun (p:pure_post a) -> pre /\ (forall (x:a). post x ==> p x))
+
+assume new type int : Type0
+
+assume HasEq_int: hasEq int
+
+assume val op_AmpAmp             : bool -> bool -> Tot bool
+assume val op_BarBar             : bool -> bool -> Tot bool
+assume val op_Negation           : bool -> Tot bool
+assume val op_Multiply           : int -> int -> Tot int
+assume val op_Subtraction        : int -> int -> Tot int
+assume val op_Addition           : int -> int -> Tot int
+assume val op_Minus              : int -> Tot int
+assume val op_LessThanOrEqual    : int -> int -> Tot bool
+assume val op_GreaterThan        : int -> int -> Tot bool
+assume val op_GreaterThanOrEqual : int -> int -> Tot bool
+assume val op_LessThan           : int -> int -> Tot bool
+assume val op_Equality :    #a:Type{hasEq a} -> a -> a -> Tot bool
+assume val op_disEquality : #a:Type{hasEq a} -> a -> a -> Tot bool
+assume new type exn : Type0
+assume new type array : Type -> Type0
+assume val strcat : string -> string -> Tot string
+
+assume HasEq_string: hasEq string
+
+type list (a:Type) =
+  | Nil  : list a
+  | Cons : hd:a -> tl:list a -> list a
+
+assume HasEq_list: (forall (a:Type).{:pattern (hasEq (list a))} hasEq a ==> hasEq (list a))
+
+type pattern =
+  | SMTPat   : #a:Type -> a -> pattern
+  | SMTPatT  : a:Type0 -> pattern
+  | SMTPatOr : list (list pattern) -> pattern
+
+assume type decreases : #a:Type -> a -> Type0
+
+(*
+   Lemma is desugared specially. You can write:
+
+     Lemma phi                 for   Lemma (requires True) phi []
+     Lemma t1..tn              for   Lemma unit t1..tn
+*)
+effect Lemma (a:Type) (pre:Type) (post:Type) (pats:list pattern) =
+       Pure a pre (fun r -> post)
+
+
+type option (a:Type) =
+  | None : option a
+  | Some : v:a -> option a
+
+assume HasEq_option: (forall (a:Type).{:pattern (hasEq (option a))} hasEq a ==> hasEq (option a))
+
+type either 'a 'b =
+  | Inl : v:'a -> either 'a 'b
+  | Inr : v:'b -> either 'a 'b
+
+assume HasEq_either: (forall (a:Type) (b:Type).{:pattern (hasEq (either a b))} (hasEq a /\ hasEq b) ==> hasEq (either a b))
+
+type result (a:Type) =
+  | V   : v:a -> result a
+  | E   : e:exn -> result a
+  | Err : msg:string -> result a
+
+(* This new bit for Dijkstra Monads for Free; it has a "double meaning",
+ * either as an alias for reasoning about the direct definitions, or as a marker
+ * for places where a CPS transformation should happen. *)
+effect M (a:Type) = Tot a
+
+assume HasEq_result: (forall (a:Type).{:pattern (hasEq (result a))} hasEq a ==> hasEq (result a))
+
+new_effect DIV = PURE
+sub_effect PURE ~> DIV  = purewp_id
+
+effect Div (a:Type) (pre:pure_pre) (post:pure_post a) =
+       DIV a
+           (fun (p:pure_post a) -> pre /\ (forall a. pre /\ post a ==> p a)) (* WP *)
+
+effect Dv (a:Type) =
+     DIV a (fun (p:pure_post a) -> (forall (x:a). p x))
+
+
+let st_pre_h  (heap:Type)          = heap -> GTot Type0
+let st_post_h (heap:Type) (a:Type) = a -> heap -> GTot Type0
+let st_wp_h   (heap:Type) (a:Type) = st_post_h heap a -> Tot (st_pre_h heap)
+
+inline let st_return        (heap:Type) (a:Type)
+                            (x:a) (p:st_post_h heap a) =
+     p x
+inline let st_bind_wp       (heap:Type)
+			    (r1:range)
+			    (a:Type) (b:Type)
+                            (wp1:st_wp_h heap a)
+                            (wp2:(a -> GTot (st_wp_h heap b)))
+                            (p:st_post_h heap b) (h0:heap) =
+     labeled r1 "push" unit
+     /\ wp1 (fun a h1 ->
+       labeled r1 "pop" unit
+       /\ wp2 a p h1) h0
+inline let st_if_then_else  (heap:Type) (a:Type) (p:Type)
+                             (wp_then:st_wp_h heap a) (wp_else:st_wp_h heap a)
+                             (post:st_post_h heap a) (h0:heap) =
+     l_ITE p
+        (wp_then post h0)
+	(wp_else post h0)
+inline let st_ite_wp        (heap:Type) (a:Type)
+                            (wp:st_wp_h heap a)
+                            (post:st_post_h heap a) (h0:heap) =
+     forall (k:st_post_h heap a).
+	 (forall (x:a) (h:heap).{:pattern (guard_free (k x h))} k x h <==> post x h)
+	 ==> wp k h0
+inline let st_stronger  (heap:Type) (a:Type) (wp1:st_wp_h heap a)
+                        (wp2:st_wp_h heap a) =
+     (forall (p:st_post_h heap a) (h:heap). wp1 p h ==> wp2 p h)
+
+inline let st_close_wp      (heap:Type) (a:Type) (b:Type)
+                             (wp:(b -> GTot (st_wp_h heap a)))
+                             (p:st_post_h heap a) (h:heap) =
+     (forall (b:b). wp b p h)
+inline let st_assert_p      (heap:Type) (a:Type) (p:Type)
+                             (wp:st_wp_h heap a)
+                             (q:st_post_h heap a) (h:heap) =
+     p /\ wp q h
+inline let st_assume_p      (heap:Type) (a:Type) (p:Type)
+                             (wp:st_wp_h heap a)
+                             (q:st_post_h heap a) (h:heap) =
+     p ==> wp q h
+inline let st_null_wp       (heap:Type) (a:Type)
+                             (p:st_post_h heap a) (h:heap) =
+     (forall (x:a) (h:heap). p x h)
+inline let st_trivial       (heap:Type) (a:Type)
+                             (wp:st_wp_h heap a) =
+     (forall h0. wp (fun r h1 -> True) h0)
+
+new_effect {
+  STATE_h (heap:Type) : result:Type -> wp:st_wp_h heap result -> Effect
+  with return_wp      = st_return heap
+     ; bind_wp      = st_bind_wp heap
+     ; if_then_else = st_if_then_else heap
+     ; ite_wp       = st_ite_wp heap
+     ; stronger     = st_stronger heap
+     ; close_wp     = st_close_wp heap
+     ; assert_p     = st_assert_p heap
+     ; assume_p     = st_assume_p heap
+     ; null_wp      = st_null_wp heap
+     ; trivial      = st_trivial heap
+}
+
+(* Effect EXCEPTION *)
+let ex_pre  = Type0
+let ex_post (a:Type) = result a -> GTot Type0
+let ex_wp   (a:Type) = ex_post a -> GTot ex_pre
+inline let ex_return   (a:Type) (x:a) (p:ex_post a) : GTot Type0 = p (V x)
+inline let ex_bind_wp (r1:range) (a:Type) (b:Type)
+		       (wp1:ex_wp a)
+		       (wp2:(a -> GTot (ex_wp b))) (p:ex_post b)
+         : GTot Type0 =
+  forall (k:ex_post b).
+     (forall (rb:result b).{:pattern (guard_free (k rb))} k rb <==> p rb)
+     ==> (labeled r1 "push" unit
+         /\ wp1 (fun ra1 -> labeled r1 "pop" unit
+			/\ (is_V ra1 ==> wp2 (V.v ra1) k)
+			/\ (is_E ra1 ==> k (E (E.e ra1)))))
+
+inline let ex_ite_wp (a:Type) (wp:ex_wp a) (post:ex_post a) =
+  forall (k:ex_post a).
+     (forall (rb:result a).{:pattern (guard_free (k rb))} k rb <==> post rb)
+     ==> wp k
+
+inline let ex_if_then_else (a:Type) (p:Type) (wp_then:ex_wp a) (wp_else:ex_wp a) (post:ex_post a) =
+   l_ITE p
+       (wp_then post)
+       (wp_else post)
+inline let ex_stronger (a:Type) (wp1:ex_wp a) (wp2:ex_wp a) =
+        (forall (p:ex_post a). wp1 p ==> wp2 p)
+
+inline let ex_close_wp (a:Type) (b:Type) (wp:(b -> GTot (ex_wp a))) (p:ex_post a) = (forall (b:b). wp b p)
+inline let ex_assert_p (a:Type) (q:Type) (wp:ex_wp a) (p:ex_post a) = (q /\ wp p)
+inline let ex_assume_p (a:Type) (q:Type) (wp:ex_wp a) (p:ex_post a) = (q ==> wp p)
+inline let ex_null_wp (a:Type) (p:ex_post a) = (forall (r:result a). p r)
+inline let ex_trivial (a:Type) (wp:ex_wp a) = wp (fun r -> True)
+
+new_effect {
+  EXN : result:Type -> wp:ex_wp result -> Effect
+  with
+    return_wp    = ex_return
+  ; bind_wp      = ex_bind_wp
+  ; if_then_else = ex_if_then_else
+  ; ite_wp       = ex_ite_wp
+  ; stronger     = ex_stronger
+  ; close_wp     = ex_close_wp
+  ; assert_p     = ex_assert_p
+  ; assume_p     = ex_assume_p
+  ; null_wp      = ex_null_wp
+  ; trivial      = ex_trivial
+}
+effect Exn (a:Type) (pre:ex_pre) (post:ex_post a) =
+       EXN a
+         (fun (p:ex_post a) -> pre /\ (forall (r:result a). (pre /\ post r) ==> p r)) (* WP *)
+
+inline let lift_div_exn (a:Type) (wp:pure_wp a) (p:ex_post a) = wp (fun a -> p (V a))
+sub_effect DIV ~> EXN = lift_div_exn
+effect Ex (a:Type) = Exn a True (fun v -> True)
+
+let all_pre_h  (h:Type)           = h -> GTot Type0
+let all_post_h (h:Type) (a:Type)  = result a -> h -> GTot Type0
+let all_wp_h   (h:Type) (a:Type)  = all_post_h h a -> Tot (all_pre_h h)
+
+inline let all_ite_wp (heap:Type) (a:Type)
+                      (wp:all_wp_h heap a)
+                      (post:all_post_h heap a) (h0:heap) =
+    forall (k:all_post_h heap a).
+       (forall (x:result a) (h:heap).{:pattern (guard_free (k x h))} k x h <==> post x h)
+       ==> wp k h0
+inline let all_return  (heap:Type) (a:Type) (x:a) (p:all_post_h heap a) = p (V x)
+inline let all_bind_wp (heap:Type) (r1:range) (a:Type) (b:Type)
+                       (wp1:all_wp_h heap a)
+                       (wp2:(a -> GTot (all_wp_h heap b)))
+                       (p:all_post_h heap b) (h0:heap) : GTot Type0 =
+   labeled r1 "push" unit
+   /\ wp1 (fun ra h1 ->
+       labeled r1 "pop" unit
+       /\ (is_V ra ==> wp2 (V.v ra) p h1)) h0
+
+inline let all_if_then_else (heap:Type) (a:Type) (p:Type)
+                             (wp_then:all_wp_h heap a) (wp_else:all_wp_h heap a)
+                             (post:all_post_h heap a) (h0:heap) =
+   l_ITE p
+       (wp_then post h0)
+       (wp_else post h0)
+inline let all_stronger (heap:Type) (a:Type) (wp1:all_wp_h heap a)
+                        (wp2:all_wp_h heap a) =
+    (forall (p:all_post_h heap a) (h:heap). wp1 p h ==> wp2 p h)
+
+inline let all_close_wp (heap:Type) (a:Type) (b:Type)
+                         (wp:(b -> GTot (all_wp_h heap a)))
+                         (p:all_post_h heap a) (h:heap) =
+    (forall (b:b). wp b p h)
+inline let all_assert_p (heap:Type) (a:Type) (p:Type)
+                         (wp:all_wp_h heap a) (q:all_post_h heap a) (h:heap) =
+    p /\ wp q h
+inline let all_assume_p (heap:Type) (a:Type) (p:Type)
+                         (wp:all_wp_h heap a) (q:all_post_h heap a) (h:heap) =
+    p ==> wp q h
+inline let all_null_wp (heap:Type) (a:Type)
+                        (p:all_post_h heap a) (h0:heap) =
+    (forall (a:result a) (h:heap). p a h)
+inline let all_trivial (heap:Type) (a:Type) (wp:all_wp_h heap a) =
+    (forall (h0:heap). wp (fun r h1 -> True) h0)
+
+new_effect {
+  ALL_h (heap:Type) : a:Type -> wp:all_wp_h heap a -> Effect
+  with
+    return_wp    = all_return       heap
+  ; bind_wp      = all_bind_wp      heap
+  ; if_then_else = all_if_then_else heap
+  ; ite_wp       = all_ite_wp       heap
+  ; stronger     = all_stronger     heap
+  ; close_wp     = all_close_wp     heap
+  ; assert_p     = all_assert_p     heap
+  ; assume_p     = all_assume_p     heap
+  ; null_wp      = all_null_wp      heap
+  ; trivial      = all_trivial      heap
+}
+
+
+
+
+
+type lex_t =
+  | LexTop  : lex_t
+  | LexCons : #a:Type -> a -> lex_t -> lex_t
+
+(* 'a * 'b *)
+type tuple2 'a 'b =
+  | Mktuple2: _1:'a
+           -> _2:'b
+           -> tuple2 'a 'b
+
+assume HasEq_tuple2: (forall (a:Type) (b:Type).{:pattern (hasEq (tuple2 a b))} (hasEq a /\ hasEq b) ==> hasEq (tuple2 a b))
+
+(* 'a * 'b * 'c *)
+type tuple3 'a 'b 'c =
+  | Mktuple3: _1:'a
+           -> _2:'b
+           -> _3:'c
+          -> tuple3 'a 'b 'c
+
+assume HasEq_tuple3: (forall (a:Type) (b:Type) (c:Type).{:pattern (hasEq (tuple3 a b c))} (hasEq a /\ hasEq b /\ hasEq c) ==> hasEq (tuple3 a b c))
+
+(* 'a * 'b * 'c * 'd *)
+type tuple4 'a 'b 'c 'd =
+  | Mktuple4: _1:'a
+           -> _2:'b
+           -> _3:'c
+           -> _4:'d
+           -> tuple4 'a 'b 'c 'd
+
+assume HasEq_tuple4: (forall (a:Type) (b:Type) (c:Type) (d:Type).{:pattern (hasEq (tuple4 a b c d))} (hasEq a /\ hasEq b /\ hasEq c /\ hasEq d) ==> hasEq (tuple4 a b c d))
+
+(* 'a * 'b * 'c * 'd * 'e *)
+type tuple5 'a 'b 'c 'd 'e =
+  | Mktuple5: _1:'a
+           -> _2:'b
+           -> _3:'c
+           -> _4:'d
+           -> _5:'e
+           -> tuple5 'a 'b 'c 'd 'e
+
+assume HasEq_tuple5: (forall (a:Type) (b:Type) (c:Type) (d:Type) (e:Type).{:pattern (hasEq (tuple5 a b c d e))} (hasEq a /\ hasEq b /\ hasEq c /\ hasEq d /\ hasEq e) ==> hasEq (tuple5 a b c d e))
+
+(* 'a * 'b * 'c * 'd * 'e * 'f *)
+type tuple6 'a 'b 'c 'd 'e 'f =
+  | Mktuple6: _1:'a
+           -> _2:'b
+           -> _3:'c
+           -> _4:'d
+           -> _5:'e
+           -> _6:'f
+           -> tuple6 'a 'b 'c 'd 'e 'f
+
+assume HasEq_tuple6: (forall (a:Type) (b:Type) (c:Type) (d:Type) (e:Type) (f:Type).{:pattern (hasEq (tuple6 a b c d e f))} (hasEq a /\ hasEq b /\ hasEq c /\ hasEq d /\ hasEq e /\ hasEq f) ==> hasEq (tuple6 a b c d e f))
+
+(* 'a * 'b * 'c * 'd * 'e * 'f * 'g *)
+type tuple7 'a 'b 'c 'd 'e 'f 'g =
+  | Mktuple7: _1:'a
+           -> _2:'b
+           -> _3:'c
+           -> _4:'d
+           -> _5:'e
+           -> _6:'f
+           -> _7:'g
+           -> tuple7 'a 'b 'c 'd 'e 'f 'g
+
+assume HasEq_tuple7: (forall (a:Type) (b:Type) (c:Type) (d:Type) (e:Type) (f:Type) (g:Type).{:pattern (hasEq (tuple7 a b c d e f g))} (hasEq a /\ hasEq b /\ hasEq c /\ hasEq d /\ hasEq e /\ hasEq f /\ hasEq g) ==> hasEq (tuple7 a b c d e f g))
+
+(* 'a * 'b * 'c * 'd * 'e * 'f * 'g * 'h *)
+type tuple8 'a 'b 'c 'd 'e 'f 'g 'h =
+  | Mktuple8: _1:'a
+           -> _2:'b
+           -> _3:'c
+           -> _4:'d
+           -> _5:'e
+           -> _6:'f
+           -> _7:'g
+           -> _8:'h
+           -> tuple8 'a 'b 'c 'd 'e 'f 'g 'h
+
+assume HasEq_tuple8: (forall (a:Type) (b:Type) (c:Type) (d:Type) (e:Type) (f:Type) (g:Type) (h:Type).{:pattern (hasEq (tuple8 a b c d e f g h))} (hasEq a /\ hasEq b /\ hasEq c /\ hasEq d /\ hasEq e /\ hasEq f /\ hasEq g /\ hasEq h) ==> hasEq (tuple8 a b c d e f g h))
+
+(* Concrete syntax (x:a & y:b x & c x y) *)
+type dtuple3 (a:Type)
+             (b:(a -> GTot Type))
+             (c:(x:a -> b x -> GTot Type)) =
+   | Mkdtuple3:_1:a
+             -> _2:b _1
+             -> _3:c _1 _2
+             -> dtuple3 a b c
+
+(* Concrete syntax (x:a & y:b x & z:c x y & d x y z) *)
+type dtuple4 (a:Type)
+             (b:(x:a -> GTot Type))
+             (c:(x:a -> b x -> GTot Type))
+             (d:(x:a -> y:b x -> z:c x y -> GTot Type)) =
+ | Mkdtuple4:_1:a
+           -> _2:b _1
+           -> _3:c _1 _2
+           -> _4:d _1 _2 _3
+           -> dtuple4 a b c d
+
+let as_requires (#a:Type) (wp:pure_wp a)  = wp (fun x -> True)
+let as_ensures  (#a:Type) (wp:pure_wp a) (x:a) = ~ (wp (fun y -> (y=!=x)))
+
+val fst : ('a * 'b) -> Tot 'a
+let fst x = Mktuple2._1 x
+
+val snd : ('a * 'b) -> Tot 'b
+let snd x = Mktuple2._2 x
+
+val dfst : #a:Type -> #b:(a -> GTot Type) -> dtuple2 a b -> Tot a
+let dfst #a #b t = Mkdtuple2._1 t
+
+val dsnd : #a:Type -> #b:(a -> GTot Type) -> t:dtuple2 a b -> Tot (b (Mkdtuple2._1 t))
+let dsnd #a #b t = Mkdtuple2._2 t
+
+assume val _assume : p:Type -> unit -> Pure unit (requires (True)) (ensures (fun x -> p))
+assume val admit   : #a:Type -> unit -> Admit a
+assume val magic   : #a:Type -> unit -> Tot a
+irreducible val unsafe_coerce  : #a:Type -> #b: Type -> a -> Tot b
+let unsafe_coerce #a #b x = admit(); x
+assume val admitP  : p:Type -> Pure unit True (fun x -> p)
+assume val _assert : p:Type -> unit -> Pure unit (requires p) (ensures (fun x -> True))
+assume val cut     : p:Type -> Pure unit (requires p) (fun x -> p)
+assume val qintro  : #a:Type -> #p:(a -> GTot Type) -> $f:(x:a -> Lemma (p x)) -> Lemma (forall (x:a). p x)
+assume val ghost_lemma: #a:Type -> #p:(a -> GTot Type) -> #q:(a -> unit -> GTot Type) ->
+  $f:(x:a -> Ghost unit (p x) (q x)) -> Lemma (forall (x:a). p x ==> q x ())
+assume val raise: exn -> Ex 'a       (* TODO: refine with the Exn monad *)
+
+
+val ignore: #a:Type -> a -> Tot unit
+let ignore #a x = ()
+
+type nat = i:int{i >= 0}
+type pos = i:int{i > 0}
+type nonzero = i:int{i<>0}
+
+let allow_inversion (a:Type)
+  : Pure unit (requires True) (ensures (fun x -> inversion a))
+  = ()
+
+(*    For the moment we require not just that the divisor is non-zero, *)
+(*    but also that the dividend is natural. This works around a *)
+(*    mismatch between the semantics of integer division in SMT-LIB and *)
+(*    in F#/OCaml. For SMT-LIB ints the modulus is always positive (as in *)
+(*    math Euclidian division), while for F#/OCaml ints the modulus has *)
+(*    the same sign as the dividend. Our arbitrary precision ints don't *)
+(*    quite correspond to finite precision F#/OCaml ints though, but to *)
+(*    OCaml's big_ints (for which the modulus is always positive).  So *)
+(*    we'll need to return to this point anyway, when we discuss how to *)
+(*    soundly map F* ints to something in F#/OCaml.  *)
+
+assume val op_Modulus            : int -> nonzero -> Tot int
+assume val op_Division           : nat -> nonzero -> Tot int
+
+let rec pow2 (x:nat) : Tot pos = if x = 0 then 1 else op_Multiply 2 (pow2 (x-1))
+let abs (x:int) : Tot int = if x >= 0 then x else -x
+
+assume val string_of_bool: bool -> Tot string
+assume val string_of_int: int -> Tot string
